io/MIO.Sig.Call.fst
@@ -6,5 +6,5 @@ assume val print_string2 : string -> Tot bool
 
 (** This file is replaced during linking with a file that contains the real
 implementation of the commands. **)
-let mio_call (caller:bool) (cmd:cmds) (arg:mio_sig.args cmd) : mio (mio_sig.res cmd arg) =
-  Call caller cmd arg Return
+let mio_call (c:caller) (cmd:cmds) (arg:mio_sig.args cmd) : mio (mio_sig.res cmd arg) =
+  Call c cmd arg Return
