io/case-study/Utils.fst
@@ -34,7 +34,7 @@ let did_not_respond' (h:trace) : bool =
 let rec is_opened_by_untrusted (h:trace) (fd:file_descr) : bool =
   match h with
   | [] -> false
-  | EOpenfile false _ res :: tl -> begin
+  | EOpenfile Ctx _ res :: tl -> begin
     if Inl? res && fd = Inl?.v res then true
     else is_opened_by_untrusted tl fd
   end
@@ -43,22 +43,22 @@ let rec is_opened_by_untrusted (h:trace) (fd:file_descr) : bool =
   | _ :: tl -> is_opened_by_untrusted tl fd
 
 val pi : policy_spec
-let pi h isTrusted cmd arg =
-  match isTrusted, cmd with
-  | false, Openfile -> 
+let pi h c cmd arg =
+  match c, cmd with
+  | Ctx, Openfile -> 
     let (fnm, _, _) : string * (list open_flag) * zfile_perm= arg in
     if fnm = "/temp" then true else false
-  | false, Read -> 
+  | Ctx, Read -> 
     let (fd, _) : file_descr * UInt8.t = arg in
     is_opened_by_untrusted h fd
-  | false, Close -> is_opened_by_untrusted h arg
-  | false, Access -> 
+  | Ctx, Close -> is_opened_by_untrusted h arg
+  | Ctx, Access -> 
     let (fnm, _) : string * list access_permission = arg in
     if fnm = "/temp" then true 
     else false
-  | false, Stat -> 
+  | Ctx, Stat -> 
     if arg = "/temp" then true else false
-  | true, Write -> true
+  | Prog, Write -> true
   | _ -> false
 
 val phi : policy pi
@@ -84,7 +84,7 @@ val wrote_at_least_once_to : file_descr -> trace -> bool
 let rec wrote_at_least_once_to client lt =
   match lt with
   | [] -> false
-  | EWrite true arg _::tl -> 
+  | EWrite Prog arg _::tl -> 
     let (fd, msg):file_descr*Bytes.bytes = arg in
     let fd' : file_descr = fd in
     let client' : file_descr = client in
@@ -104,9 +104,9 @@ val every_request_gets_a_response_acc : trace -> list file_descr -> Type0
 let rec every_request_gets_a_response_acc lt read_descrs =
   match lt with
   | [] -> read_descrs == []
-  | ERead true arg (Inl _) :: tl ->
+  | ERead Prog arg (Inl _) :: tl ->
     let (fd, _) = arg in every_request_gets_a_response_acc tl (fd :: read_descrs)
-  | EWrite true (fd,_) _ :: tl -> every_request_gets_a_response_acc tl (filter (fun fd' -> fd <> fd') read_descrs)
+  | EWrite Prog (fd,_) _ :: tl -> every_request_gets_a_response_acc tl (filter (fun fd' -> fd <> fd') read_descrs)
   | _ :: tl -> every_request_gets_a_response_acc tl read_descrs
 
 val every_request_gets_a_response : trace -> Type0
@@ -115,12 +115,12 @@ let every_request_gets_a_response lt =
 
 let no_write_true e =
   match e with
-  | EWrite true _ _ -> false
+  | EWrite Prog _ _ -> false
   | _ -> true
 
 let no_read_true e : GTot bool =
   match e with
-  | ERead true _ (Inl _) -> false
+  | ERead Prog _ (Inl _) -> false
   | _ -> true
 
 let ergar = every_request_gets_a_response_acc
@@ -131,22 +131,22 @@ let rec ergar_ignore_no_write_read lt e lt' rl :
     (ensures ergar (lt @ e :: lt') rl)
 = match lt with
   | [] -> ()
-  | ERead true arg (Inl _) :: tl -> 
+  | ERead Prog arg (Inl _) :: tl -> 
     let (fd, _) = arg in ergar_ignore_no_write_read tl e lt' (fd :: rl)
-  | EWrite true (fd,x) y :: tl ->
-    assert_norm (ergar (EWrite true (fd,x) y :: tl @ lt') rl == ergar (tl @ lt') (filter (fun fd' -> fd <> fd') rl)) ;
+  | EWrite Prog (fd,x) y :: tl ->
+    assert_norm (ergar (EWrite Prog (fd,x) y :: tl @ lt') rl == ergar (tl @ lt') (filter (fun fd' -> fd <> fd') rl)) ;
     ergar_ignore_no_write_read tl e lt' (filter (fun fd' -> fd <> fd') rl) ;
-    assert_norm (ergar (tl @ e :: lt') (filter (fun fd' -> fd <> fd') rl) == ergar (EWrite true (fd,x) y :: tl @ e :: lt') rl)
+    assert_norm (ergar (tl @ e :: lt') (filter (fun fd' -> fd <> fd') rl) == ergar (EWrite Prog (fd,x) y :: tl @ e :: lt') rl)
   | _ :: tl -> ergar_ignore_no_write_read tl e lt' rl
 
 let is_write_true e : GTot bool =
   match e with
-  | EWrite true _ y -> true
+  | EWrite Prog _ y -> true
   | _ -> false
 
 let write_true_fd e : Pure file_descr (requires is_write_true e) (ensures fun _ -> True) =
   match e with
-  | EWrite true arg y -> fst arg
+  | EWrite Prog arg y -> fst arg
 
 let cong (f : 'a -> 'b) (x y : 'a) :
   Lemma (requires x == y) (ensures f x == f y)
@@ -160,11 +160,11 @@ let ergar_write_true e l rl :
       ergar l (filter (fun fd' -> write_true_fd e <> fd') rl)
     )
 = match e with
-  | EWrite true (fd,x) y ->
+  | EWrite Prog (fd,x) y ->
     calc (==) {
       write_true_fd e ;
       == {}
-      write_true_fd (EWrite true (fd,x) y) ;
+      write_true_fd (EWrite Prog (fd,x) y) ;
       == {}
       fd ;
     } ;
@@ -173,7 +173,7 @@ let ergar_write_true e l rl :
     calc (==) {
       ergar (e :: l) rl ;
       == {}
-      ergar (EWrite true (fd,x) y :: l) rl ;
+      ergar (EWrite Prog (fd,x) y :: l) rl ;
       == { _ by (FStar.Tactics.compute ()) }
       ergar l (filter (fun fd' -> fd <> fd') rl) ;
       == {}
@@ -192,18 +192,18 @@ let rec ergar_merge lt rl0 rl1 rl2 :
     (ensures ergar lt (rl0 @ rl1 @ rl2))
 = match lt with
   | [] -> ()
-  | ERead true (fd,_) (Inl _) :: tl ->
+  | ERead Prog (fd,_) (Inl _) :: tl ->
     assert (ergar tl (fd :: rl0 @ rl1)) ;
     assert (ergar tl (fd :: rl0 @ rl2)) ;
     ergar_merge tl (fd :: rl0) rl1 rl2
-  | EWrite true (fd,x) y :: tl ->
-    cong (fun fd -> (fun fd' -> fd <> fd')) fd (write_true_fd (EWrite true (fd,x) y)) ;
+  | EWrite Prog (fd,x) y :: tl ->
+    cong (fun fd -> (fun fd' -> fd <> fd')) fd (write_true_fd (EWrite Prog (fd,x) y)) ;
 
-    ergar_write_true (EWrite true (fd,x) y) tl (rl0 @ rl1) ;
+    ergar_write_true (EWrite Prog (fd,x) y) tl (rl0 @ rl1) ;
     assert (ergar tl (filter (fun fd' -> fd <> fd') (rl0 @ rl1))) ;
     filter_append (fun fd' -> fd <> fd') rl0 rl1 ;
 
-    ergar_write_true (EWrite true (fd,x) y) tl (rl0 @ rl2) ;
+    ergar_write_true (EWrite Prog (fd,x) y) tl (rl0 @ rl2) ;
     assert (ergar tl (filter (fun fd' -> fd <> fd') (rl0 @ rl2))) ;
     filter_append (fun fd' -> fd <> fd') rl0 rl2 ;
 
@@ -217,7 +217,7 @@ let rec ergar_merge lt rl0 rl1 rl2 :
       filter (fun fd' -> fd <> fd') (rl0 @ rl1 @ rl2) ;
     } ;
 
-    ergar_write_true (EWrite true (fd,x) y) tl (rl0 @ rl1 @ rl2) ;
+    ergar_write_true (EWrite Prog (fd,x) y) tl (rl0 @ rl1 @ rl2) ;
     assert (ergar tl (filter (fun fd' -> fd <> fd') (rl0 @ rl1 @ rl2)))
   | _ :: tl -> ergar_merge tl rl0 rl1 rl2
 
@@ -227,24 +227,24 @@ let rec ergar_split lt rl1 rl2 :
     (ensures ergar lt rl1 /\ ergar lt rl2)
 = match lt with
   | [] -> ()
-  | ERead true (fd,_) (Inl _) :: tl ->
+  | ERead Prog (fd,_) (Inl _) :: tl ->
     assert (ergar tl (fd :: rl1 @ rl2)) ;
     ergar_split tl (fd :: rl1) rl2 ;
     assert (ergar tl (fd :: rl1)) ;
     ergar_split tl [fd] rl1 ;
     ergar_merge tl [] [fd] rl2 ;
     assert (ergar tl (fd :: rl2))
-  | EWrite true (fd,x) y :: tl ->
-    cong (fun fd -> (fun fd' -> fd <> fd')) fd (write_true_fd (EWrite true (fd,x) y)) ;
+  | EWrite Prog (fd,x) y :: tl ->
+    cong (fun fd -> (fun fd' -> fd <> fd')) fd (write_true_fd (EWrite Prog (fd,x) y)) ;
 
-    ergar_write_true (EWrite true (fd,x) y) tl (rl1 @ rl2) ;
+    ergar_write_true (EWrite Prog (fd,x) y) tl (rl1 @ rl2) ;
     assert (ergar tl (filter (fun fd' -> fd <> fd') (rl1 @ rl2))) ;
     filter_append (fun fd' -> fd <> fd') rl1 rl2 ;
 
     ergar_split tl (filter (fun fd' -> fd <> fd') rl1) (filter (fun fd' -> fd <> fd') rl2) ;
 
-    ergar_write_true (EWrite true (fd,x) y) tl rl1 ;
-    ergar_write_true (EWrite true (fd,x) y) tl rl2
+    ergar_write_true (EWrite Prog (fd,x) y) tl rl1 ;
+    ergar_write_true (EWrite Prog (fd,x) y) tl rl2
   | _ :: tl -> ergar_split tl rl1 rl2
 
 let rec filter_swap f g l :
@@ -259,7 +259,7 @@ let rec ergar_filter lt rl f :
     (ensures ergar lt (filter f rl))
 = match lt with
   | [] -> ()
-  | ERead true (fd,_) (Inl _) :: tl ->
+  | ERead Prog (fd,_) (Inl _) :: tl ->
     assert (ergar tl (fd :: rl)) ;
     ergar_filter tl (fd :: rl) f ;
     assert (ergar tl (filter f (fd :: rl))) ;
@@ -272,13 +272,13 @@ let rec ergar_filter lt rl f :
       ergar_merge tl [] [fd] (filter f rl) ;
       assert (ergar tl (fd :: filter f rl))
     end
-  | EWrite true (fd,x) y :: tl ->
-    ergar_write_true (EWrite true (fd,x) y) tl rl ;
-    cong (fun fd -> (fun fd' -> fd <> fd')) fd (write_true_fd (EWrite true (fd,x) y)) ;
+  | EWrite Prog (fd,x) y :: tl ->
+    ergar_write_true (EWrite Prog (fd,x) y) tl rl ;
+    cong (fun fd -> (fun fd' -> fd <> fd')) fd (write_true_fd (EWrite Prog (fd,x) y)) ;
     assert (ergar tl (filter (fun fd' -> fd <> fd') rl)) ;
     ergar_filter tl (filter (fun fd' -> fd <> fd') rl) f ;
     assert (ergar tl (filter f (filter (fun fd' -> fd <> fd') rl))) ;
-    ergar_write_true (EWrite true (fd,x) y) tl (filter f rl) ;
+    ergar_write_true (EWrite Prog (fd,x) y) tl (filter f rl) ;
     filter_swap (fun fd' -> fd <> fd') f rl ;
     assert (ergar tl (filter (fun fd' -> fd <> fd') (filter f rl)))
   | _ :: tl -> ergar_filter tl rl f
@@ -293,19 +293,19 @@ let rec ergar_write_irr lt e0 lt' rl :
     ergar_filter lt' rl (fun fd' -> write_true_fd e0 <> fd') ;
     ergar_write_true e0 lt' rl ;
     assert (ergar lt' (filter (fun fd' -> write_true_fd e0 <> fd') rl))
-  | ERead true (fd,_) (Inl _) :: tl ->
+  | ERead Prog (fd,_) (Inl _) :: tl ->
     assert (ergar (tl @ lt') (fd :: rl)) ;
     ergar_write_irr tl e0 lt' (fd :: rl) ;
     assert (ergar ((tl @ [ e0 ]) @ lt') (fd :: rl))
-  | EWrite true (fd,x) y :: tl ->
-    cong (fun fd -> (fun fd' -> fd <> fd')) fd (write_true_fd (EWrite true (fd,x) y)) ;
+  | EWrite Prog (fd,x) y :: tl ->
+    cong (fun fd -> (fun fd' -> fd <> fd')) fd (write_true_fd (EWrite Prog (fd,x) y)) ;
 
-    ergar_write_true (EWrite true (fd,x) y) (tl @ lt') rl ;
+    ergar_write_true (EWrite Prog (fd,x) y) (tl @ lt') rl ;
     assert (ergar (tl @ lt') (filter (fun fd' -> fd <> fd') rl)) ;
 
     ergar_write_irr tl e0 lt' (filter (fun fd' -> fd <> fd') rl) ;
 
-    ergar_write_true (EWrite true (fd,x) y) ((tl @ [e0]) @ lt') rl ;
+    ergar_write_true (EWrite Prog (fd,x) y) ((tl @ [e0]) @ lt') rl ;
     assert (ergar ((tl @ [ e0 ]) @ lt') (filter (fun fd' -> fd <> fd') rl))
   | _ :: tl -> ergar_write_irr tl e0 lt' rl
 
@@ -323,9 +323,9 @@ let rec ergar_pi_irr h lth lt lt' :
     append_assoc lt [ e ] lt' ;
     assert (every_request_gets_a_response (lt @ lt')) ;
     begin match e with
-    | EWrite true (fd,x) y ->
-      ergar_write_irr lt (EWrite true (fd,x) y) lt' [] ;
-      assert (every_request_gets_a_response ((lt @ [ EWrite true (fd,x) y ]) @ lt')) ;
+    | EWrite Prog (fd,x) y ->
+      ergar_write_irr lt (EWrite Prog (fd,x) y) lt' [] ;
+      assert (every_request_gets_a_response ((lt @ [ EWrite Prog (fd,x) y ]) @ lt')) ;
       ergar_pi_irr (e :: h) l (lt @ [ e ]) lt'
     | _ ->
       ergar_ignore_no_write_read lt e lt' [] ;
@@ -342,7 +342,7 @@ let rec ergar_pi_write_aux h lth client :
   | e :: l ->
     assert (enforced_locally pi (e :: h) l) ;
     begin match e with
-    | EWrite true (fd,x) y ->
+    | EWrite Prog (fd,x) y ->
       if fd = client
       then ergar_pi_irr (e :: h) l [] []
       else ergar_pi_write_aux (e :: h) l client
@@ -355,13 +355,13 @@ let rec ergar_trace_merge lt lt' rl rl' :
     (ensures ergar (lt @ lt') (rl @ rl'))
 = match lt with
   | [] -> ()
-  | ERead true (fd,limit) (Inl _) :: tl ->
+  | ERead Prog (fd,limit) (Inl _) :: tl ->
     assert (ergar tl (fd :: rl)) ;
     ergar_trace_merge tl lt' (fd :: rl) rl'
-  | EWrite true (fd,x) y :: tl ->
-    cong (fun fd -> (fun fd' -> fd <> fd')) fd (write_true_fd (EWrite true (fd,x) y)) ;
+  | EWrite Prog (fd,x) y :: tl ->
+    cong (fun fd -> (fun fd' -> fd <> fd')) fd (write_true_fd (EWrite Prog (fd,x) y)) ;
 
-    ergar_write_true (EWrite true (fd,x) y) tl rl ;
+    ergar_write_true (EWrite Prog (fd,x) y) tl rl ;
     assert (ergar tl (filter (fun fd' -> fd <> fd') rl)) ;
 
     assert (ergar lt' rl') ;
@@ -370,19 +370,19 @@ let rec ergar_trace_merge lt lt' rl rl' :
     filter_append (fun fd' -> fd <> fd') rl rl' ;
     ergar_trace_merge tl lt' (filter (fun fd' -> fd <> fd') rl) (filter (fun fd' -> fd <> fd') rl') ;
 
-    ergar_write_true (EWrite true (fd,x) y) (tl @ lt') (rl @ rl') ;
+    ergar_write_true (EWrite Prog (fd,x) y) (tl @ lt') (rl @ rl') ;
     assert (ergar (tl @ lt') (filter (fun fd' -> fd <> fd') (rl @ rl')))
   | _ :: tl -> ergar_trace_merge tl lt' rl rl'
 
 let ergar_pi_write h lth client limit r lt :
   Lemma
     (requires enforced_locally pi h lth /\ wrote_at_least_once_to client lth /\ every_request_gets_a_response lt)
-    (ensures every_request_gets_a_response (lt @ [ ERead true (client,limit) (Inl r) ] @ lth))
+    (ensures every_request_gets_a_response (lt @ [ ERead Prog (client,limit) (Inl r) ] @ lth))
 = ergar_pi_write_aux h lth client ;
   assert (ergar lth [client]) ;
-  assert (every_request_gets_a_response (ERead true (client,limit) (Inl r) :: lth)) ;
-  append_assoc lt [ ERead true (client,limit) (Inl r) ] lth ;
-  ergar_trace_merge lt ([ ERead true (client,limit) (Inl r) ] @ lth) [] []
+  assert (every_request_gets_a_response (ERead Prog (client,limit) (Inl r) :: lth)) ;
+  append_assoc lt [ ERead Prog (client,limit) (Inl r) ] lth ;
+  ergar_trace_merge lt ([ ERead Prog (client,limit) (Inl r) ] @ lth) [] []
 
 let every_request_gets_a_response_append () : 
   Lemma (
