io/case-study/AdversarialHandlers.fst
@@ -12,28 +12,28 @@ type tgt_handler = ctx_tgt tgt_cs_int
 
 // Does not do anything, fails postcondition
 val handler1 : tgt_handler
-let handler1 #fl io_acts client req send = Inl ()
+let handler1 #fl call_io client req send = Inl ()
 
 // Tries to `send` a too long reply
 val handler2 : tgt_handler
-let handler2 #fl io_acts client req send = send (Bytes.create 501ul 10uy) 
+let handler2 #fl call_io client req send = send (Bytes.create 501ul 10uy) 
 
 // Tries to read forbidden file
 val handler3 : ctx_tgt tgt_cs_int 
-let handler3 #fl io_acts client req send =
-  let _ = io_acts Openfile ("/etc/passwd",[O_RDWR],0x650) in
+let handler3 #fl call_io client req send =
+  let _ = call_io Openfile ("/etc/passwd",[O_RDWR],0x650) in
   Inl ()
 
 // Tries to directly write to client directly instead of using send
 val handler4 : tgt_handler
-let handler4 #fl io_acts client req send =
-  let _ = io_acts Write (client,(Bytes.create 501ul 10uy)) in
+let handler4 #fl call_io client req send =
+  let _ = call_io Write (client,(Bytes.create 501ul 10uy)) in
   Inl ()
 
 // Tries to create a socket, which is not an IO operation
 val handler5 : tgt_handler
-let handler5 #fl io_acts client req send =
-  let _ = io_acts Socket () in
+let handler5 #fl call_io client req send =
+  let _ = call_io Socket () in
   Inl ()
 
 
